examples/steel/Selectors.Examples.fst
@@ -1,6 +1,6 @@
 module Selectors.Examples
 
-open Steel.Effect.Atomic
+// open Steel.Effect.Atomic
 open Steel.Effect
 open Steel.Reference
 
@@ -8,6 +8,19 @@ open Steel.Reference
 
 #push-options "--fuel 0 --ifuel 0 --ide_id_info_off"
 
+module T = FStar.Tactics
+
+#set-options "--print_full_names --log_queries"
+
+let debug(r r':ref int) : Steel unit
+  (vptr r `star` vptr r') (fun _ -> vptr r `star` vptr r')
+  (requires fun _ -> True)
+  (ensures fun _ _ h1 -> sel r h1 == 0)
+  by (T.norm normal_steps; T.dump "here")
+  = write r 1;
+    write r 0
+
+(*
 let swap (#a:Type0) (r1 r2:ref a) : Steel unit
   (vptr r1 `star` vptr r2)
   (fun _ -> vptr r1 `star` vptr r2)
@@ -62,3 +75,4 @@ let test3 (r1 r2 r3:ref int) : Steel unit
     assert (sel r1 h1 == 1);
     assert (sel r2 h0 == sel r2 h1);
     write r1 0
+*)
